Partial fixes to flattened bug and TM soundness issue

Source/DafnyStandardLibraries/examples/Actions/ActionsExamples.dfy
@@ -4,10 +4,11 @@ module ActionsExamples {
   import opened Std.Consumers
   import opened Std.Wrappers
   import opened Std.Frames
+  import opened Std.Termination
 
   // Demonstrating the simplest idiom
   // for looping over the values produced by a Producer<T>
-  method SimpleProducerLoop() {
+  method {:test} SimpleProducerLoop() {
     var p := MakeProducer();
     while true
       invariant p.Valid()
@@ -19,6 +20,7 @@ module ActionsExamples {
         break;
       }
 
+      print "Got: ", next.value, "\n";
       expect 0 <= next.value < 5;
     }
   }
@@ -137,5 +139,131 @@ module ActionsExamples {
     var _ := a.Invoke(5);
     assert a.Inputs() == [1, 2, 3, 4, 5];
     assert a.storage.items == [1, 2, 3, 4, 5];
+  }
+
+  twostate predicate FooTest(b: Box) reads {} {
+    && fresh(b)
+    && Foo(b)
+    && Foo2(b)
+  }
+
+  predicate Foo(b: Box)
+    reads b
+  {
+    b.i == 42
+  }
+
+  twostate predicate Foo2(new b: Box)
+    reads b
+  {
+    b.i == 42
+  }
+
+  @AssumeCrossModuleTermination
+  // TODO: This should be expressible as Mapped(Seq(inputs), Split)
+  class SplitProducer extends Producer<Producer<nat>>, ProducesNewProducersProof<nat> {
+
+    var inputs: seq<nat>
+
+    constructor (inputs: seq<nat>)
+      ensures Valid()
+      ensures fresh(Repr)
+      ensures history == []
+    {
+      this.inputs := inputs;
+
+      history := [];
+      Repr := {this};
+      height := 1;
+      remainingMetric := TMNat(|inputs|);
+    }
+
+    ghost predicate Valid()
+      reads this, Repr
+      ensures Valid() ==> this in Repr
+      ensures Valid() ==> ValidHistory(history)
+      decreases height, 0
+    {
+      && this in Repr
+      && ValidHistory(history)
+      && remainingMetric == TMNat(|inputs|)
+      && (0 < |inputs| ==> Seq.All(Outputs(), IsSome))
+    }
+
+    twostate function DumbRepr(new o: Producer<nat>): set<object>
+      reads o
+    {
+      o.Repr
+    }
+
+    twostate predicate ValidOutput(history: seq<((), Option<Producer<nat>>)>, nextInput: (), new nextOutput: Option<Producer<nat>>)
+      decreases height
+      ensures ValidOutput(history, nextInput, nextOutput) ==> ValidHistory(history + [(nextInput, nextOutput)])
+    {
+      ValidHistory(history + [(nextInput, nextOutput)])
+    }
+    ghost predicate ValidOutputs(outputs: seq<Option<Producer<nat>>>)
+      requires Seq.Partitioned(outputs, IsSome)
+      decreases height
+    {
+      true
+    }
+
+    method Invoke(t: ()) returns (result: Option<Producer<nat>>)
+      requires Requires(t)
+      reads Repr
+      modifies Modifies(t)
+      decreases Decreases(t).Ordinal(), 0
+      ensures Ensures(t, result)
+      ensures if result.Some? then 
+          old(remainingMetric).DecreasesTo(remainingMetric)
+        else
+          old(remainingMetric) == remainingMetric
+    {
+      if inputs == [] {
+        result := None;
+
+        OutputsPartitionedAfterOutputtingNone();
+        ProduceNone();
+      } else {
+        var x := inputs[0];
+        inputs := Seq.DropFirst(inputs);
+        var p := new SeqReader([x / 2, x - (x / 2)]);
+        
+        result := Some(p);
+
+        OutputsPartitionedAfterOutputtingSome(result.value);
+        ProduceSome(result.value);
+      }
+
+      remainingMetric := TMNat(|inputs|);
+      reveal TerminationMetric.DecreasesTo();
+    }
+
+    ghost function Producer(): Producer<Producer<nat>> {
+      this
+    }
+
+    // TODO: Depends on figuring out the reads clause issues with ValidOutput
+    twostate lemma {:axiom} ProducedAllNew(new produced: Producer<nat>)
+      requires old(Action().Valid())
+      requires Action().ValidOutput(old(Action().history), (), Some(produced))
+      ensures produced.Valid()
+      ensures fresh(produced.Repr)
+      ensures produced.history == []
+  }
+
+  @IsolateAssertions
+  method {:test} ExamplePipeline() {
+    var producerProducer := new SplitProducer([1, 2, 3, 4, 5]);
+
+    var flattened := new FlattenedProducer(producerProducer, producerProducer);
+    
+    var collector := new SeqWriter();
+
+    var collectorTotalProof := new DefaultTotalActionProof(collector);
+    flattened.ForEachRemaining(collector, collectorTotalProof);
+    
+    expect collector.values == [0, 1, 1, 1, 1, 2, 2, 2, 2, 3], collector.values;
   }
 }
